LeanProjeto2/TestesAndOthers/SoundnessAjudas.lean
@@ -1,0 +1,6 @@
+/- IGUALDADE ENTRE UNIV CLOSURE OF BASE AND ITS CORRESP AXIOMS
+lemma AxS4_eq (x₁ x₂ : String) : (∀₁₁ x₁ (AxiomS4_matrix x₁ x₂) = (AxiomS4 x₁ x₂)) :=
+by
+  unfold AxiomS4
+  rfl
+-/
